---
layout: default
title: Standard notations and common functions
categories: clrs
---

### Solution 3.2-1
Given $f(n)$ and $g(n)$ are monotonically increasing. For any $a > b$, we have $f(a) \geq f(b)$ and $g(a) \geq g(b)$. 

By adding the equations, we have $f(a) + g(a) \geq f(b) + g(b)$. Or, $f(n) + g(n)$ is also monotonically increasing.

We also have $f(g(a)) \geq f(g(b))$ as $g(a) \geq g(b)$. Hence, $f(g(n))$ is monotonically increasing.

And finally, if $f$ and $g$ are non negative, $f(a) \cdot g(a) \geq f(b) \cdot g(b)$. And we have $f(n) \cdot g(n)$ is monotonically increasing.

### Solution 3.2-2
To prove, $a^{\log\_b c} = c^{\log\_b a}$. Let, 
\\begin{align\*}
x & = a^{\log\_b c} \\\\\\
\lg x & = \log\_b c \cdot \lg a \\\\\\
& = \dfrac{\lg c}{\lg b} \cdot \lg a \\\\\\
& = \dfrac{\lg a}{\lg b} \cdot \lg c \\\\\\
& = \log\_b a \cdot \lg c \\\\\\
x & = c^{\log\_b a}
\\end{align\*}

### Solution 3.2-3
Using Stirling's approximation,
\\begin{align\*}
n! & = \sqrt{2\pi n} \bigg(\frac{n}{e}\bigg)^n \bigg(1 + \Theta\Big(\frac{1}{n}\Big) \bigg) \\\\\\
\lg n! & = \lg \bigg(\sqrt{2\pi n} \bigg(\frac{n}{e}\bigg)^n \bigg(1 + \Theta\Big(\frac{1}{n}\Big) \bigg) \bigg) \\\\\\
& = \lg\Big(\sqrt{2\pi n}\Big) + n \lg (n/e) + \lg \bigg(1 + \Theta\Big(\frac{1}{n}\Big)\bigg) \\\\\\
& = \Theta(\sqrt n) + \Theta(n \lg n) + \lg (\Theta(1) + \Theta(1/n)) \\\\\\
& = \Theta(n \lg n)
\\end{align\*} 

Now let's prove $n! = o(n^n)$
\\begin{align\*}
n! & = n \cdot (n - 1) \ldots 2 \cdot 1  \\\\\\
& < n \cdot n \ldots n \\\\\\
& = n^n \\\\\\
& = o(n^n)
\\end{align\*} 

Also, let's prove $n! = \omega (2^n)$
\\begin{align\*}
n! & = n \cdot (n - 1) \ldots 2 \cdot 1  \\\\\\
& > 2 \cdot 2 \ldots 2 \\\\\\
& = 2^n \\\\\\
& = \omega(2^n)
\\end{align\*} 

### Soltion 3.2-4
From Stirling's approximation, $\lg n! = \Theta(n \lg n)$. Let's use $n = (\lg n)! $, that is
\\begin{align\*}
\lg (\lg n)! & = \Theta (\lg n \lg \lg n) \\\\\\
& = \omega (\lg n) \\\\\\
\lg (\lg n)! & > k \lg n \\\\\\
(\lg n)! & > n^k && \mbox{ for any } k
\\end{align\*}
Hence, $(\lg n)!$ is no polynomially bounded. 

Now, let $n = (\lg \lg n)!$,
\\begin{align\*}
\lg (\lg \lg n)! & = \Theta (\lg \lg n \lg \lg \lg n) \\\\\\
& = o((\lg \lg n)^2) \\\\\\
& = o(\lg n) \\\\\\
& < k \lg n \\\\\\
(\lg \lg n)! & < n^k
\\end{align\*}
Hence, $(\lg \lg n)!$ is polynomially bounded. 

### Solution 3.2-5
$ \lg^\*(\lg{n}) = \lg^\*n - 1 > \lg(\lg^\*(n)) $. So $ \lg^\*(\lg{n}) $ 
is asymptotically larger than $\lg(\lg^\*(n))$. 

Let $m = \lg^\* n$, and assume that $n \geq 4$. Hence $\lg^\*(\lg n) = m - 1$. 
We are now comparing between $\lg (\lg^\* n) = \lg m$ and $m - 1$. 
Clearly $m - 1$ is asymptotically larger than $\lg m$ when $m$ is 
sufficiently large. Thus we can conclude that $\lg^\* (\lg n)$ is 
asymptotically larger than $\lg(\lg^\*n)$.

### Solution 3.2-6
Just substituting the value of $\phi$ and $\hat{\phi}$ in the equation gives the solution directly.

### Solution 3.2-7
Base case: $i = 0$. $F\_0 = \dfrac{1 -1 }{\sqrt{5}} = 0$ and $i = 1$, 
$F\_1 = \dfrac{\phi - \hat{\phi}}{\sqrt{5}} = 1 $.

Induction hypothesis: For $i = 2,3,\ldots,(n-1)$, $F_i$ holds good.

Inductive step:
\\begin{align\*}
F\_n & = F\_{n - 1} + F\_{n - 2} \\\\\\
 & = \dfrac{\phi^{n - 1} - \hat{\phi}^{n - 1}}{\sqrt{5}} + \dfrac{\phi^{n - 2} - \hat{\phi}^{n - 2}}{\sqrt{5}} \\\\\\
& = \dfrac{\phi^{n-2} (\phi + 1) - \hat{\phi}^{n-2} (\hat{\phi} + 1) }{\sqrt{5}} \\\\\\
& = \dfrac{\phi^{n-2} (\phi^2) - \hat{\phi}^{n-2} (\hat{\phi}^2) }{\sqrt{5}} \\\\\\
& = \dfrac{\phi^{n} - \hat{\phi}^{n}}{\sqrt{5}}
\\end{align\*}
Hence, proved. 

### Solution 3.2-8
We are given $k \ln k = \Theta(n)$. By reflexivity of $\Theta$, we have, $\Theta(k \ln k) = n$.
\\begin{align\*}
n & = \Theta(k \ln k) \\\\\\
\ln n & = \Theta(\ln (k \ln n)) \\\\\\
& = \Theta(\ln k + \ln \ln n) \\\\\\
& = \Theta(\ln k) \\\\\\
\dfrac{n}{\ln n} & = \dfrac{\Theta(k \ln k)}{\Theta(\ln k)} = \Theta(k) \\\\\\
k & = \Theta(n/\ln n )
\\end{align\*}
Hence, proved. 